Change stack model to proj_/inj_value instead of encode/decode
This patch changes to using proj_value/inj_value instead of encode/decode
for the stack as well as the register file. This should help with copying
bytes (that must be Fragments to be meaningful) between the stack and
registers, ensuring that they are interpreted equivalently.

backend/Locations.v
@@ -344,7 +344,7 @@ Module Stack.
     Mem.getN (Z.to_nat (AST.typesize (typ_of_quantity q))) (addr ofs) (stack sl).
 
   Definition get sl ofs q (stack: t) : val :=
-    decode_val (chunk_of_type (typ_of_quantity q)) (get_bytes sl ofs q stack).
+    proj_value q (get_bytes sl ofs q stack).
 
   Definition set_bytes sl ofs (bytes: list memval) (stack: t) : t :=
     fun slot =>
@@ -354,13 +354,13 @@ Module Stack.
         stack slot.
 
   Definition set sl ofs q (v: val) (stack: t) : t :=
-    set_bytes sl ofs (encode_val (chunk_of_type (typ_of_quantity q)) v) stack.
+    set_bytes sl ofs (inj_value q v) stack.
 
   Lemma chunk_length:
-    forall ty v,
-    Z.to_nat (AST.typesize ty) = length (encode_val (chunk_of_type ty) v).
+    forall q v,
+    Z.to_nat (AST.typesize (typ_of_quantity q)) = length (inj_value q v).
   Proof.
-    intros. rewrite encode_val_length. destruct ty; auto.
+    intros. rewrite inj_value_length. destruct q; auto.
   Qed.
 
   Lemma gss:
@@ -369,8 +369,10 @@ Module Stack.
   Proof.
     intros. unfold get, set, get_bytes, set_bytes.
     rewrite dec_eq_true. erewrite chunk_length. rewrite Mem.getN_setN_same.
-    erewrite <- decode_encode_val_similar; eauto.
-    eapply decode_encode_val_general.
+    destruct (Val.has_type_dec v (typ_of_quantity q)).
+    - rewrite proj_inj_value, Val.load_result_same; auto.
+      destruct q; auto.
+    - destruct q, v; simpl in *; intuition auto.
   Qed.
 
   Lemma gso:
