backend/LTLtyping.v
@@ -115,8 +115,19 @@ Lemma well_typed_locset:
   forall ls, wt_locset ls.
 Proof.
   unfold wt_locset, Locmap.get, Locmap.chunk_of_loc. intros.
-  rewrite <- type_of_chunk_of_type.
-  destruct ls. destruct l; apply decode_val_type.
+  destruct ls, l.
+  - simpl. unfold Regfile.get, Regfile.quantity_of_mreg, Regfile.chunk_of_mreg.
+    destruct (mreg_type_cases r); rewrite H; simpl.
+    exploit proj_value_fits_quantity; intro.
+    generalize fits_quantity_Q32; intros [A B]; eauto.
+    exploit proj_value_fits_quantity; intro.
+    generalize fits_quantity_Q64; intros [A B]; eauto.
+  - simpl. unfold Stack.get.
+    destruct q.
+    exploit proj_value_fits_quantity; intro.
+    generalize fits_quantity_Q32; intros [A B]; eauto.
+    exploit proj_value_fits_quantity; intro.
+    generalize fits_quantity_Q64; intros [A B]; eauto.
 Qed.
 
 (** Soundness of the type system *)
